cequiv/approx_props2.v
@@ -1,6 +1,8 @@
 (*
 
   Copyright 2014 Cornell University
+  Copyright 2015 Cornell University
+  Copyright 2016 Cornell University
 
   This file is part of VPrl (the Verified Nuprl project).
 
@@ -18,7 +20,10 @@
   along with VPrl.  If not, see <http://www.gnu.org/licenses/>.
 
 
-  Website: http://nuprl.org/html/verification/
+  Websites: http://nuprl.org/html/verification/
+            http://nuprl.org/html/Nuprl2Coq
+            https://github.com/vrahli/NuprlInCoq
+
   Authors: Abhishek Anand & Vincent Rahli
 
 *)
@@ -162,3 +167,10 @@ Proof.
   allrw remove_nvars_nil_l; allrw app_nil_r.
   allrw subvars_app_l; sp.
 Qed.
+
+
+(*
+*** Local Variables:
+*** coq-load-path: ("." "../util/" "../terms/" "../computation/")
+*** End:
+*)
