cequiv/domain_th.v
@@ -2,6 +2,7 @@
 
   Copyright 2014 Cornell University
   Copyright 2015 Cornell University
+  Copyright 2016 Cornell University
 
   This file is part of VPrl (the Verified Nuprl project).
 
@@ -19,7 +20,10 @@
   along with VPrl.  If not, see <http://www.gnu.org/licenses/>.
 
 
-  Website: http://nuprl.org/html/verification/
+  Websites: http://nuprl.org/html/verification/
+            http://nuprl.org/html/Nuprl2Coq
+            https://github.com/vrahli/NuprlInCoq
+
   Authors: Abhishek Anand & Vincent Rahli
 
 *)
@@ -8317,14 +8321,14 @@ Proof.
 Qed.
 
 Lemma sqlen_rel_rw_seq {o} :
-  forall lib (f fv e : @NTerm o) v s,
+  forall lib k (f fv e : @NTerm o) v s,
     reduces_to lib f fv
     -> isprogram f
     -> isprogram (apply_bterm (bterm [v] e) [mk_fix f])
     -> computes_to_seq lib (apply_bterm (bterm [v] e) [mk_fix f]) s
     -> {s' : ntseq
         $ computes_to_seq lib (apply_bterm (bterm [v] e) [mk_fix fv]) s'
-        # (forall n, alpha_eq (s n) (s' n)) }.
+        # (forall n, sqle_n lib k (s n) (s' n)) }.
 Proof.
   introv Hred Hprf Hpr Hcv.
   duplicate Hred as Hc.
@@ -8332,9 +8336,11 @@ Proof.
   simpl in Hpr0.
   eapply reduces_to_subst_fix in Hc; eauto.
   repnud Hc.
-  clear Hc. rename Hc0 into Hap.
+  clear Hc.
+  rename Hc0 into Hap.
   apply approx_sqle in Hap.
-  specialize (Hap (S 0)). invertsn Hap.
+  specialize (Hap (S k)).
+  invertsn Hap.
   repnud Hap; GC.
   apply Hap4 in Hcv; exrepnd.
   clear Hap2 Hap3 Hap4.
@@ -8641,7 +8647,7 @@ forall k : nat,
           eapply hasvalue_approx; eauto with slow. }
 
     { allunfold @computes_to_value; repnd.
-      eapply sqlen_rel_rw_seq in Hcvb0; try (exact Hred); auto; exrepnd.
+      eapply (sqlen_rel_rw_seq _ 1) in Hcvb0; try (exact Hred); auto; exrepnd.
       clear Hcvb1.
 
       pose proof (weaker_crary_5_8 lib t' e (sterm s')) as h; simpl in h.
@@ -8716,7 +8722,7 @@ forall k : nat,
           eapply hasvalue_approx; eauto with slow. }
 
     { allunfold @computes_to_value; repnd.
-      eapply sqlen_rel_rw_seq in Hcvb0; try (exact Hred); auto; exrepnd.
+      eapply (sqlen_rel_rw_seq _ 1) in Hcvb0; try (exact Hred); auto; exrepnd.
       clear Hcvb1.
 
       pose proof (weaker_crary_5_8_isp_can_or_exc lib (mk_exception a e0) e (sterm s')) as h; simpl in h.
@@ -9231,7 +9237,7 @@ Lemma crary_5_9_really_aux_seq {o} :
                                   (apply_bterm (bterm [nvarx] e) [fix_approx k f]))
                         -> {s' : ntseq
                             $ computes_to_seq lib t s'
-                            # (forall n, alpha_eq (s n) (s' n))}.
+                            # (forall n, sqle_n lib mm (s n) (s' n))}.
 Proof.
     intros lib mm IHmm t e XX Hispbt s f Hp XX0 Hcvb Hub1 e2' Hcv1 Hcv2 j Hcv3.
     rename Hcv3 into Hapa.
@@ -9266,6 +9272,12 @@ Proof.
     exrepnd.
     exists f'; dands; auto.
     introv; eauto 3 with slow.
+    pose proof (H0a1 n) as q.
+    apply howetheorem1 in q; eauto 3 with slow.
+    apply approx_sqle in q.
+    specialize (q mm).
+    eapply (fst (respects_alpha_sqlen _ _));[|exact q].
+    eauto 3 with slow.
 Qed.
 
 (* end hide *)
@@ -9462,7 +9474,7 @@ Proof.
       duplicate XX0 as XXb.
       apply (apply_bterm_fix_program_rw _ _ _ _ Hcv1) in XX0; auto.
 
-      eapply sqlen_rel_rw_seq in comp; eauto; exrepnd.
+      eapply (sqlen_rel_rw_seq _ mm) in comp; eauto; exrepnd.
       apply reduces_to_implies_cequiv in Hcv1; auto. clear Hub.
       apply (cequiv_approx_ub_rw _ _ _ _ _ Hcv1) in Hubbb.
       rename Hubbb into Hub1.
@@ -9487,12 +9499,14 @@ Proof.
       eexists; dands; eauto.
       introv; eauto 3 with slow.
 
+      eapply sqlen_n_trans; eauto.
+
     + repnud Hcv; exrepnd.
       repnud Hcv1.
       duplicate XX0 as XXb.
       apply (apply_bterm_fix_program_rw _ _ _ _ Hcv1) in XX0; auto.
 
-      eapply sqlen_rel_rw_seq in comp; eauto; exrepnd.
+      eapply (sqlen_rel_rw_seq _ mm) in comp; eauto; exrepnd.
       apply reduces_to_implies_cequiv in Hcv1; auto. clear Hub.
       apply (cequiv_approx_ub_rw _ _ _ _ _ Hcv1) in Hubbb.
       rename Hubbb into Hub1.
@@ -9518,6 +9532,8 @@ Proof.
       exrepnd.
       eexists; dands; eauto.
       introv; eauto 3 with slow.
+
+      eapply sqlen_n_trans; eauto.
 
     + exrepnd.
       applydup @computes_to_seq_implies_computes_to_value in comp as comp'; eauto 3 with slow;[].
@@ -9565,6 +9581,7 @@ Lemma cequiv_approximations: forall f g s t,
 Proof.
   introv Hpf Hpg Hint.
 *)
+
 
 (*
 *** Local Variables:
